theories/heap_lang/adequacy.v
@@ -6,13 +6,13 @@ Set Default Proof Using "Type".
 
 Class heapPreG Σ := HeapPreG {
   heap_preG_iris :> invPreG Σ;
-  heap_preG_heap :> gen_heapPreG loc val Σ;
-  heap_preG_inv_heap :> inv_heapPreG loc val Σ;
+  heap_preG_heap :> gen_heapPreG loc (option val) Σ;
+  heap_preG_inv_heap :> inv_heapPreG loc (option val) Σ;
   heap_preG_proph :> proph_mapPreG proph_id (val * val) Σ;
 }.
 
 Definition heapΣ : gFunctors :=
-  #[invΣ; gen_heapΣ loc val; inv_heapΣ loc val; proph_mapΣ proph_id (val * val)].
+  #[invΣ; gen_heapΣ loc (option val); inv_heapΣ loc (option val); proph_mapΣ proph_id (val * val)].
 Instance subG_heapPreG {Σ} : subG heapΣ Σ → heapPreG Σ.
 Proof. solve_inG. Qed.
 
@@ -22,7 +22,7 @@ Definition heap_adequacy Σ `{!heapPreG Σ} s e σ φ :
 Proof.
   intros Hwp; eapply (wp_adequacy _ _); iIntros (??) "".
   iMod (gen_heap_init σ.(heap)) as (?) "Hh".
-  iMod (inv_heap_init loc val) as (?) ">Hi".
+  iMod (inv_heap_init loc (option val)) as (?) ">Hi".
   iMod (proph_map_init κs σ.(used_proph_id)) as (?) "Hp".
   iModIntro. iExists
     (λ σ κs, (gen_heap_ctx σ.(heap) ∗ proph_map_ctx κs σ.(used_proph_id))%I),
